spec/lean/Oak.lean
@@ -97,6 +97,7 @@ import Oak.Stdlib.PercentLaws
 import Oak.Stdlib.PercentStrictLaws
 import Oak.Stdlib.Base32Laws
 import Oak.Stdlib.Base64StrictLaws
+import Oak.Stdlib.Base32StrictLaws
 import Oak.Stdlib.RandomLaws
 import Oak.Stdlib.UuidLaws
 import Oak.Stdlib.HashLaws
